# $\displaystyle{\sum_{i=1}^{n}\frac{1}{i}} = \sum_{i=1}^{n}(-1)^{i-1}\frac{1}{i}\binom{n}{i}$

差分法证明，记右式为$f(n)$，左式为$g(n)$。 $$\begin{aligned}
        f(n+1) - f(n) &= \displaystyle \sum_{i = 1}^{n+1} (-1)^{i-1} \frac{1}{i}\binom{n+1}{i} - \sum_{i=1}^{n}(-1)^{i-1}\frac{1}{i}\binom{n}{i} \\
        &= \displaystyle \sum_{i=1}^{n+1}(-1)^{i-1} \frac{1}{i}(\binom{n}{i} + \binom{n}{i-1}) - \sum_{i=1}^{n}(-1)^{i-1}\frac{1}{i}\binom{n}{i} \\
        &= \displaystyle \sum_{i=1}^{n+1}(-1)^{i-1} \frac{1}{i} \binom{n}{i-1} + (-1)^{n+1} \frac{1}{n+1} \binom{n}{n+1}\\
        &= \displaystyle \sum_{i=0}^{n}(-1)^i \frac{1}{i+1} \binom{n}{i} + 0 \\
        &= \displaystyle \sum_{i=0}^{n+1}(-1)^i \frac{1}{i+1} \binom{n}{i} \\ 
    
\end{aligned}$$
通过差分将上式化为比较简单的式子，接下来处理每一项中的$\frac{1}{i+1}$部分，注意到
$$\begin{aligned}
        \frac{1}{i+1} \binom{n}{i} &= \frac{1}{i+1} \frac{n!}{(n-i)!i!} \\
        &= \frac{n!}{(n-i)!(i+1)!} \\
        &= \frac{(n+1)!}{(n-i)!(i+1)!} \frac{1}{n+1} \\
        &= \binom{n+1}{i+1} \frac{1}{n+1}
    
\end{aligned}$$ 
代回，得 $$\begin{aligned}
        f(n+1) - f(n) &= \displaystyle \sum_{i=0}^{n+1}(-1)^i \frac{1}{i+1} \binom{n}{i} \\ 
        &= \displaystyle \sum_{i=0}^{n+1}(-1)^i \frac{1}{n+1} \binom{n+1}{i+1} \\
        &= \displaystyle \frac{1}{n+1} (\sum_{i=1}^{n+2} (-1)^{i-1} \binom{n+1}{i} -1 + 1)\\
        &= \displaystyle \frac{1}{n+1} (\sum_{i=1}^{n+1} (-1)^{i-1} \binom{n+1}{i} + (-1)^{-1}\binom{n+1}{0} +1)\\
        &= \displaystyle \frac{1}{n+1} (\sum_{i=0}^{n+1} (-1)^{i-1} \binom{n+1}{i} + 1)\\
        &= \displaystyle \frac{1}{n+1} (-\sum_{i=0}^{n+1}\binom{n+1}{i} (-1)^i 1^{n+1-i} + 1) \\
        &= \displaystyle \frac{1}{n+1} (-(-1+1)^{n+1} + 1) \\
        &= \displaystyle \frac{1}{n+1}. 
    
\end{aligned}$$

因此有$f(n+1) - f(n) = g(n+1) - g(n)$.

考虑$n = 1$时，$f(1) = g(1) = 1$.

所以$f(n) = g(n)$。

QED.
